Make progress with cv translation of compiler backend

cv_translator/backend_arm8_cvScript.sml
@@ -148,4 +148,328 @@ QED
 val _ = cv_auto_trans (arm8_targetTheory.arm8_enc_def |>
                        SRULE [combinTheory.o_DEF, LIST_BIND_def, FUN_EQ_THM]);
 
+(*---------------------------------------------------------------------------*
+  Translation of instruction encoder
+ *---------------------------------------------------------------------------*)
+
+(* generic *)
+
+val _ = cv_trans sptreeTheory.fromAList_def;
+
+val _ = cv_trans lab_to_targetTheory.lab_inst_def;
+val _ = cv_auto_trans lab_to_targetTheory.get_ffi_index_def;
+val _ = cv_auto_trans lab_to_targetTheory.find_pos_def;
+val _ = cv_auto_trans lab_to_targetTheory.get_label_def;
+val _ = cv_trans lab_to_targetTheory.pad_bytes_def;
+val _ = cv_auto_trans lab_filterTheory.filter_skip_def;
+val _ = cv_auto_trans lab_to_targetTheory.prog_to_bytes_def;
+val _ = cv_auto_trans lab_to_targetTheory.zero_labs_acc_exist_def;
+val _ = cv_auto_trans lab_to_targetTheory.find_ffi_names_def;
+val _ = TypeBase.accessors_of “:lab_to_target$inc_config” |> map cv_trans;
+val _ = TypeBase.accessors_of “:environment” |> map cv_trans;
+
+val _ = cv_trans num_list_enc_decTheory.append_rev_def;
+
+Triviality make_cv_term_provable:
+  (if n < 30 then x else y) = (if n = 0n then x else if 30 ≤ n then y else x)
+Proof
+  rw [] \\ gvs []
+QED
+
+val pre = cv_trans_pre $
+  SRULE [make_cv_term_provable] num_list_enc_decTheory.num_to_chars_def;
+
+Theorem num_to_chars_pre[cv_pre,local]:
+  ∀n. num_to_chars_pre n
+Proof
+  completeInduct_on ‘n’ \\ simp [Once pre] \\ rw []
+  \\ ‘n MOD 30 < 30’ by gs [] \\ decide_tac
+QED
+
+val _ = cv_trans num_list_enc_decTheory.rev_nums_to_chars_def;
+
+Triviality spt_enc_def[cv_inline] = num_list_enc_decTheory.spt_enc_def;
+
+val _ = cv_auto_trans backend_enc_decTheory.data_to_word_config_enc_def;
+val _ = cv_auto_trans backend_enc_decTheory.word_to_word_config_enc_def;
+val _ = cv_auto_trans backend_enc_decTheory.word_to_stack_config_enc_def;
+val _ = cv_auto_trans backend_enc_decTheory.stack_to_lab_config_enc_def;
+val _ = cv_auto_trans backend_enc_decTheory.lab_to_target_inc_config_enc_def;
+val _ = cv_auto_trans backend_enc_decTheory.tap_config_enc_def;
+
+(* environment encoding *)
+
+val tms = backend_enc_decTheory.environment_enc_def
+            |> concl |> find_terms (can (match_term “namespace_enc _”)) |> map rand;
+val tm1 = el 1 tms;
+val tm2 = el 2 tms;
+
+fun spec_namespace_enc' tm1 suffix = let
+  val name = "namespace_enc'" ^ suffix
+  val name_list = "namespace_enc'" ^ suffix ^ "_list"
+  val r = “namespace_enc' ^tm1”
+  val r_list = “namespace_enc'_list ^tm1”
+  val v = mk_var(name,type_of r)
+  val v_list = mk_var(name_list,type_of r_list)
+  val tm = num_list_enc_decTheory.namespace_enc'_def
+    |> CONJUNCTS |> map (ISPEC tm1 o Q.GEN ‘e’ o SPEC_ALL) |> LIST_CONJ |> SRULE [LET_THM]
+    |> concl |> subst [r |-> v, r_list |-> v_list]
+  val tac =  WF_REL_TAC ‘measure (λx. case x of
+                         | INL x => namespace_size (K 0) (K 0) (K 0) x
+                         | INR x => namespace1_size (K 0) (K 0) (K 0) x)’
+  val def = tDefine name [ANTIQUOTE tm] tac
+  val _ = cv_auto_trans def
+  val cs = def |> CONJUNCTS |> map (fst o strip_comb o lhs o concl o SPEC_ALL)
+  val c = hd cs
+  val c_list = last cs
+  val goal = mk_conj(mk_eq(r,c),mk_eq(r_list,c_list))
+  val res = prove(goal,
+                  simp [FUN_EQ_THM]
+                  \\ ho_match_mp_tac (fetch "-" (name ^ "_ind"))
+                  \\ simp [def,num_list_enc_decTheory.namespace_enc'_def])
+  in res end
+
+val res1 = spec_namespace_enc' tm1 "_1";
+val res2 = spec_namespace_enc' tm2 "_2";
+
+val _ = cv_trans num_list_enc_decTheory.namespace_depth_def;
+
+val _ = cv_trans (backend_enc_decTheory.environment_enc_def
+                    |> SRULE [res1,res2,num_list_enc_decTheory.namespace_enc_def,
+                              num_list_enc_decTheory.prod_enc_def]);
+
+val _ = cv_auto_trans backend_enc_decTheory.source_to_flat_config_enc_def;
+
+(* closLang const encoding *)
+
+val const_exp = backend_enc_decTheory.const_enc'_def
+                |> SRULE [SF ETA_ss, num_tree_enc_decTheory.list_enc'_def];
+val const_exps = MAP |> CONJUNCTS |> map (Q.ISPEC ‘const_enc'’);
+
+val name = "const_enc_aux"
+val c = “const_enc'”
+val r = mk_var(name,type_of c)
+val c_list = “MAP const_enc'”
+val r_list = mk_var(name ^ "_list",type_of c_list)
+
+Definition const_enc_aux_def:
+  ^(LIST_CONJ (CONJUNCTS const_exp @ const_exps |> map SPEC_ALL)
+           |> concl |> subst [c|->r,c_list|->r_list])
+End
+
+val _ = cv_auto_trans const_enc_aux_def;
+
+Theorem const_enc_aux_thm[cv_inline,local]:
+  const_enc' = const_enc_aux ∧
+  MAP const_enc' = const_enc_aux_list
+Proof
+  gvs [FUN_EQ_THM] \\ Induct
+  \\ gvs [const_enc_aux_def,backend_enc_decTheory.const_enc'_def,
+          num_tree_enc_decTheory.list_enc'_def,SF ETA_ss]
+QED
+
+(* bvl_exp encoding *)
+
+val bvl_exp = backend_enc_decTheory.bvl_exp_enc'_def
+                |> SRULE [SF ETA_ss, num_tree_enc_decTheory.list_enc'_def];
+val bvl_exps = MAP |> CONJUNCTS |> map (Q.ISPEC ‘bvl_exp_enc'’);
+
+val name = "bvl_exp_enc_aux"
+val c = “bvl_exp_enc'”
+val r = mk_var(name,type_of c)
+val c_list = “MAP bvl_exp_enc'”
+val r_list = mk_var(name ^ "_list",type_of c_list)
+
+Definition bvl_exp_enc_aux_def:
+  ^(LIST_CONJ (CONJUNCTS bvl_exp @ bvl_exps |> map SPEC_ALL)
+           |> concl |> subst [c|->r,c_list|->r_list])
+End
+
+val _ = cv_auto_trans bvl_exp_enc_aux_def;
+
+Theorem bvl_exp_enc_aux_thm[cv_inline,local]:
+  bvl_exp_enc' = bvl_exp_enc_aux ∧
+  MAP bvl_exp_enc' = bvl_exp_enc_aux_list
+Proof
+  gvs [FUN_EQ_THM] \\ Induct
+  \\ gvs [bvl_exp_enc_aux_def,backend_enc_decTheory.bvl_exp_enc'_def,
+          num_tree_enc_decTheory.list_enc'_def,SF ETA_ss]
+QED
+
+val _ = cv_auto_trans backend_enc_decTheory.bvl_to_bvi_config_enc_def;
+
+(* closLang_exp encoding *)
+
+val closLang_exp = backend_enc_decTheory.closLang_exp_enc'_def
+                |> SRULE [SF ETA_ss, num_tree_enc_decTheory.list_enc'_def];
+val closLang_exps = MAP |> CONJUNCTS |> map (Q.ISPEC ‘closLang_exp_enc'’);
+val closLang_exps1 = MAP |> CONJUNCTS |> map (Q.ISPEC ‘pair_enc' num_enc' closLang_exp_enc'’);
+
+val name = "closLang_exp_enc_aux"
+val c = “closLang_exp_enc'”
+val r = mk_var(name,type_of c)
+val c_list = “MAP closLang_exp_enc'”
+val r_list = mk_var(name ^ "_list",type_of c_list)
+val c_list1 = “MAP $ pair_enc' num_enc' closLang_exp_enc'”
+val r_list1 = mk_var(name ^ "_list1",type_of c_list1)
+
+Definition closLang_exp_enc_aux_def:
+  ^(CONJUNCTS closLang_exp @ closLang_exps @ closLang_exps1
+    |> map (SPEC_ALL o SIMP_RULE bool_ss [FORALL_PROD,
+              num_tree_enc_decTheory.pair_enc'_def]) |> LIST_CONJ
+    |> concl |> subst [c|->r,c_list|->r_list,c_list1|->r_list1])
+Termination
+  WF_REL_TAC ‘measure $ λx. case x of
+              | INL x => closLang$exp_size x
+              | INR (INL xs) => list_size closLang$exp_size xs
+              | INR (INR ys) => list_size (pair_size (λx.x) closLang$exp_size) ys’
+  \\ gvs [closLangTheory.exp_size_eq]
+End
+
+val pre = cv_auto_trans_pre closLang_exp_enc_aux_def;
+
+Theorem closLang_exp_enc_aux_pre[cv_pre,local]:
+  (∀v. closLang_exp_enc_aux_pre v) ∧
+  (∀v. closLang_exp_enc_aux_list_pre v) ∧
+  (∀v. closLang_exp_enc_aux_list1_pre v)
+Proof
+  ho_match_mp_tac closLang_exp_enc_aux_ind \\ rw [] \\ simp [Once pre]
+QED
+
+Theorem closLang_exp_enc_aux_thm[cv_inline,local]:
+  closLang_exp_enc' = closLang_exp_enc_aux ∧
+  MAP closLang_exp_enc' = closLang_exp_enc_aux_list ∧
+  MAP (pair_enc' num_enc' closLang_exp_enc') = closLang_exp_enc_aux_list1
+Proof
+  gvs [FUN_EQ_THM] \\ ho_match_mp_tac closLang_exp_enc_aux_ind
+  \\ gvs [closLang_exp_enc_aux_def,SF ETA_ss,
+          backend_enc_decTheory.closLang_exp_enc'_def,
+          num_tree_enc_decTheory.pair_enc'_def,
+          num_tree_enc_decTheory.list_enc'_def]
+QED
+
+(* closLang val_approx encoding *)
+
+val val_approx_exp = backend_enc_decTheory.val_approx_enc'_def
+                |> SRULE [SF ETA_ss, num_tree_enc_decTheory.list_enc'_def];
+val val_approx_exps = MAP |> CONJUNCTS |> map (Q.ISPEC ‘val_approx_enc'’);
+
+val name = "val_approx_enc_aux"
+val c = “val_approx_enc'”
+val r = mk_var(name,type_of c)
+val c_list = “MAP val_approx_enc'”
+val r_list = mk_var(name ^ "_list",type_of c_list)
+
+Definition val_approx_enc_aux_def:
+  ^(LIST_CONJ (CONJUNCTS val_approx_exp @ val_approx_exps |> map SPEC_ALL)
+           |> concl |> subst [c|->r,c_list|->r_list])
+End
+
+val _ = cv_auto_trans val_approx_enc_aux_def;
+
+Theorem val_approx_enc_aux_thm[cv_inline,local]:
+  val_approx_enc' = val_approx_enc_aux ∧
+  MAP val_approx_enc' = val_approx_enc_aux_list
+Proof
+  gvs [FUN_EQ_THM] \\ Induct
+  \\ gvs [val_approx_enc_aux_def,backend_enc_decTheory.val_approx_enc'_def,
+          num_tree_enc_decTheory.list_enc'_def,SF ETA_ss]
+QED
+
+val _ = cv_auto_trans backend_enc_decTheory.clos_to_bvl_config_enc_def;
+
+val _ = cv_auto_trans backend_enc_decTheory.inc_config_enc_def;
+val _ = cv_trans backend_enc_decTheory.encode_backend_config_def;
+val _ = cv_auto_trans backend_asmTheory.attach_bitmaps_def;
+
+(* 64-bit *)
+
+val arch_spec = INST_TYPE [alpha |-> “:64”];
+
+val _ = cv_trans (alignmentTheory.aligned_w2n |> arch_spec);;
+val _ = cv_trans (asmTheory.offset_ok_def |> arch_spec);
+val _ = cv_trans (lab_to_targetTheory.section_labels_def |> arch_spec);
+val _ = cv_trans (lab_to_targetTheory.compute_labels_alt_def |> arch_spec);
+val _ = cv_trans (lab_to_targetTheory.lines_upd_lab_len_def |> arch_spec);
+
+val pre = cv_trans_pre (lab_to_targetTheory.upd_lab_len_def |> arch_spec);
+
+Theorem upd_lab_len_pre[cv_pre]:
+  ∀pos v. upd_lab_len_pre pos v
+Proof
+  Induct_on ‘v’ \\ simp [Once pre]
+QED
+
+val _ = cv_trans (lab_to_targetTheory.add_nop_def |> arch_spec);
+
+val pre = cv_trans_pre (lab_to_targetTheory.pad_section_def |> arch_spec);
+
+Theorem pad_section_pre[cv_pre,local]:
+  ∀nop v aux. pad_section_pre nop v aux
+Proof
+  Induct_on ‘v’ \\ simp [Once pre]
+QED
+
+val _ = cv_trans (lab_to_targetTheory.pad_code_def |> arch_spec);
+
+(* arm8 specific *)
+
+Triviality fp_reg_ok_arm8_def[cv_inline] = fp_reg_ok_arm8_def;
+
+val _ = cv_auto_trans inst_ok_arm8_def;
+val _ = cv_auto_trans asm_ok_arm8_def;
+val _ = cv_auto_trans line_ok_light_arm8_def;
+val _ = cv_auto_trans sec_ok_light_arm8_def;
+val _ = cv_auto_trans (lab_to_targetTheory.get_jump_offset_def |> arch_spec);
+
+val pre = cv_trans_pre enc_lines_again_arm8_def;
+
+Theorem enc_lines_again_arm8_pre[cv_pre,local]:
+  ∀labs ffis pos v0 v. enc_lines_again_arm8_pre labs ffis pos v0 v
+Proof
+  Induct_on ‘v0’ \\ simp [Once pre]
+QED
+
+val pre = cv_trans_pre enc_secs_again_arm8_def;
+
+Theorem enc_secs_again_arm8_pre[cv_pre,local]:
+  ∀pos labs ffis v. enc_secs_again_arm8_pre pos labs ffis v
+Proof
+  Induct_on ‘v’ \\ simp [Once pre]
+QED
+
+val pre = cv_auto_trans_pre remove_labels_loop_arm8_def;
+
+Theorem remove_labels_loop_arm8_pre[cv_pre]:
+  ∀clock pos init_labs ffis sec_list.
+    remove_labels_loop_arm8_pre clock pos init_labs ffis sec_list
+Proof
+  Induct_on ‘clock’ \\ simp [Once pre]
+QED
+
+val _ = cv_trans enc_line_arm8_def;
+val _ = cv_auto_trans enc_sec_arm8_def;
+val _ = cv_auto_trans enc_sec_list_arm8_def;
+val _ = cv_trans remove_labels_arm8_def;
+val _ = cv_auto_trans compile_lab_arm8_def;
+val _ = cv_trans lab_to_target_arm8_def;
+val _ = cv_trans from_lab_arm8_def;
+
+(* ----------------------------------------------------------------------------------- *)
+
+(*
+stack_to_labTheory.compile_def
+
+from_stack_arm8_def
+from_word_arm8_def
+from_word_0_arm8_def
+get_forced_arm8_def
+word_alloc_inlogic_arm8_def
+each_inlogic_arm8_def
+word_to_word_inlogic_arm8_def
+to_word_0_arm8_def
+compile_0_arm8_def |> SRULE [data_to_wordTheory.stubs_def]
+compile_cake_arm8_def
+*)
+
 val _ = export_theory();
