cv_translator/README.md
@@ -2,39 +2,3 @@ Translator to cv type used by cv_compute
 
 [backend_arm8_cvScript.sml](backend_arm8_cvScript.sml):
 Translate cv version of arm8 specialised backend functions.
-
-[cv_bootScript.sml](cv_bootScript.sml):
-Apply cv translator to bootstrap example from HOL
-
-[cv_demoScript.sml](cv_demoScript.sml):
-Demo use of cv translator
-
-[cv_golScript.sml](cv_golScript.sml):
-Sketch of symbolic conway's game-of-life evaluation
-
-[cv_memLib.sml](cv_memLib.sml):
-The cv translator's state is handled by this Lib file
-
-[cv_miscLib.sml](cv_miscLib.sml):
-Miscellaneous functions used in cv automation
-
-[cv_primScript.sml](cv_primScript.sml):
-Prove theorems cv_transLib uses for its operation
-
-[cv_repLib.sml](cv_repLib.sml):
-Derives cv_rep theorems (which cv_transLib uses internally).
-
-[cv_repScript.sml](cv_repScript.sml):
-Define cv_rep and prove a few lemmas used in proof automation
-
-[cv_stdScript.sml](cv_stdScript.sml):
-Apply cv translator to standard theories list, pair, sptree, etc.
-
-[cv_transLib.sml](cv_transLib.sml):
-Main entry points to the cv translator
-
-[cv_typeLib.sml](cv_typeLib.sml):
-Automation for defining translations into and out of cv type
-
-[cv_typeScript.sml](cv_typeScript.sml):
-Definitions and theorems that support cv_typeLib
